tree_map false specification

trees.v
@@ -18,11 +18,13 @@ Fixpoint in_order {X : Type} (t : tree X) : list X :=
   end
 .
 
+Definition leaf {X : Type} (x : X) := (node empty x empty).
+
 Definition example_tree : tree nat := (
   node
-    (node (node empty 1 empty) 3 (node empty 2 empty))
+    (node (leaf 1) 3 (leaf 2))
     0
-    (node (node empty 4 empty) 1 (node empty 5 empty))
+    (node (leaf 4) 1 (leaf 5))
   )
 .
 
@@ -40,9 +42,9 @@ Fixpoint tree_map {X Y} (f : X -> Y) (t : tree X) : tree Y :=
 Example tree_map_example_1 :
   tree_map (fun x => [x; 2 * x]) example_tree = (
     node
-      (node (node empty [1; 2] empty) [3; 6] (node empty [2; 4] empty))
+      (node (leaf [1; 2]) [3; 6] (leaf [2; 4]))
       [0; 0]
-      (node (node empty [4; 8] empty) [1; 2] (node empty [5; 10] empty))
+      (node (leaf [4; 8]) [1; 2] (leaf [5; 10]))
   ).
 Proof. reflexivity. Qed.
 
@@ -64,8 +66,8 @@ Proof.
     reflexivity.
 Qed.
 
-Definition injective {A B} (f : A -> B) :=
-  forall x y : A, f x = f y -> x = y.
+Definition injective {X Y : Type} (f : X -> Y) :=
+  forall x y : X, f x = f y -> x = y.
 
 Theorem tree_map_injective : forall {X Y : Type} (f : X -> Y),
   injective f -> injective (tree_map f).
@@ -93,3 +95,158 @@ Proof.
     reflexivity.
 Qed.
 *)
+
+Fixpoint search_tree_rec (t : tree nat) : Prop :=
+  match t with
+  | empty => True
+  | node l x r => (
+    let search_tree_l := search_tree_rec l in
+    let l_less_than := match l with
+      | empty => True
+      | node ll lx lr => lx <= x
+    end in
+    let search_tree_r := search_tree_rec r in
+    let less_than_r := match l with
+      | empty => True
+      | node rl rx rr => x <= rx
+    end in
+    search_tree_l /\ l_less_than /\ search_tree_r /\ less_than_r
+  )
+  end
+.
+
+Inductive search_tree : tree nat -> Prop :=
+  | SearchTree_Empty : search_tree empty
+  | SearchTree_Node (l : tree nat) (x : nat) (r : tree nat) :
+    search_tree_left x l -> search_tree_right x r -> search_tree (node l x r)
+    (*
+    let p := search_tree (node l x r) in
+    match l, r return p with
+    | empty, empty => p
+    | node ll lx lr, empty => lx <= x -> p
+    | empty, node rl rx rr => x <= rx -> p
+    | node ll lx lr, node rl rx rr => lx <= x -> x <= rx -> p
+    end
+    *)
+
+with search_tree_left : nat -> tree nat -> Prop :=
+  | SearchTree_Left_Empty (x : nat) : search_tree_left x empty
+  | SearchTree_Left_Node (x : nat) (ll : tree nat) (lx : nat) (lr : tree nat) :
+    let l := node ll lx lr in
+    search_tree l -> lx <= x -> search_tree_left x l
+
+with search_tree_right : nat -> tree nat -> Prop :=
+  | SearchTree_Right_Empty (x : nat) : search_tree_right x empty
+  | SearchTree_Right_Node (x : nat) (rl : tree nat) (rx : nat) (rr : tree nat) :
+    let r := node rl rx rr in
+    search_tree r -> x <= rx -> search_tree_right x r
+.
+
+Theorem leaf_search_tree : forall (x : nat),
+  search_tree (leaf x).
+Proof.
+  intros; unfold leaf.
+  apply SearchTree_Node.
+  - apply SearchTree_Left_Empty.
+  - apply SearchTree_Right_Empty.
+Qed.
+
+Example search_tree_ex_1 : search_tree (
+  node
+    (node (node (leaf 2) 4 (leaf 5)) 4 (leaf 6))
+    7
+    (node empty 7 (leaf 10))
+).
+Proof.
+  apply SearchTree_Node.
+  - apply SearchTree_Left_Node.
+    + apply SearchTree_Node.
+      * apply SearchTree_Left_Node.
+        -- apply SearchTree_Node.
+          ++ apply SearchTree_Left_Node.
+            ** apply leaf_search_tree.
+            ** apply le_S. apply le_S. apply le_n.
+          ++ apply SearchTree_Right_Node.
+            ** apply leaf_search_tree.
+            ** apply le_S. apply le_n.
+        -- apply le_n.
+      * apply SearchTree_Right_Node.
+        -- apply leaf_search_tree.
+        -- apply le_S. apply le_S. apply le_n.
+    + apply le_S. apply le_S. apply le_S. apply le_n.
+  - apply SearchTree_Right_Node.
+    + apply SearchTree_Node.
+      * apply SearchTree_Left_Empty.
+      * apply SearchTree_Right_Node.
+        -- apply leaf_search_tree.
+        -- apply le_S. apply le_S. apply le_S. apply le_n.
+    + apply le_n.
+Qed.
+
+Definition search_tree_neg_1 := node (leaf 5) 8 (leaf 6).
+
+Example search_tree_ex_neg_1 : ~search_tree search_tree_neg_1.
+Proof.
+  unfold not; intros.
+  inversion H; subst. inversion H4; subst.
+  rename H7 into H_le. repeat (
+    inversion H_le as [n | n H_le' H_n_eq]; subst;
+    clear H_le; rename H_le' into H_le
+  ).
+Qed.
+
+Theorem dist_exists_not_all : forall {X : Type} (P : X -> Prop),
+  (exists (x : X), ~ P x) -> ~(forall (x : X), P x).
+Proof.
+  unfold not; intros X P H_exists_x_not_Px H_forall_x_Px.
+  destruct H_exists_x_not_Px as [x H_not_Px].
+  apply H_not_Px. apply H_forall_x_Px.
+Qed.
+
+Theorem not_imp_imp_and : forall (P Q : Prop),
+  P /\ ~Q -> ~(P -> Q).
+Proof.
+  unfold not; intros P Q H H_P_imp_Q; destruct H as [H_P H_not_Q].
+  apply H_not_Q. apply H_P_imp_Q. apply H_P.
+Qed.
+
+Definition f_const {X Y : Type} (x : X) :=
+  fun (y : Y) => x.
+
+Theorem search_tree_const : forall (x : nat) (t : tree nat),
+  search_tree (tree_map (f_const x) t).
+Proof.
+  intros. induction t as [| l IHl tx r IHr]; simpl.
+  - apply SearchTree_Empty.
+  - apply SearchTree_Node.
+    + destruct l; simpl.
+      * apply SearchTree_Left_Empty.
+      * apply SearchTree_Left_Node.
+        -- apply IHl.
+        -- unfold f_const. apply le_n.
+    + destruct r; simpl.
+      * apply SearchTree_Right_Empty.
+      * apply SearchTree_Right_Node.
+        -- apply IHr.
+        -- unfold f_const. apply le_n.
+Qed.
+
+Theorem tree_map_search_tree_counter_ex :
+  exists (f : nat -> nat) (t : tree nat),
+  search_tree (tree_map f t) /\ ~(search_tree t).
+Proof.
+  exists (f_const 0). exists search_tree_neg_1. split.
+  - apply search_tree_const.
+  - exact search_tree_ex_neg_1.
+Qed.
+
+Theorem tree_map_search_tree_not_implies_search_tree :
+  ~(forall (f : nat -> nat) (t : tree nat),
+    search_tree (tree_map f t) -> search_tree t).
+Proof.
+  pose (H_counter_ex := tree_map_search_tree_counter_ex).
+  destruct H_counter_ex as [f [t H_counter]].
+  apply dist_exists_not_all. exists f.
+  apply dist_exists_not_all. exists t.
+  apply not_imp_imp_and. exact H_counter.
+Qed.
